formalization/ListCtx.v
@@ -1,0 +1,541 @@
+From stdpp Require Import mapset.
+From CT Require Import Atom.
+From CT Require Import NamelessTactics.
+From Coq Require Import Lists.List.
+Import Atom.
+Import Tactics.
+Import NamelessTactics.
+Import List.
+
+(** This file defines an ordered type context used in refinement typing. *)
+
+(** Type Context Definition (Γ in Fig. 4) *)
+(** We use list instead of set since the type context in the refinement typing has dependency. *)
+Definition listctx (A: Type) := list (atom * A).
+
+Fixpoint ctxdom {A: Type} (Γ: listctx A) : aset :=
+  match Γ with
+  | [] => ∅
+  | (x, _) :: Γ => {[x]} ∪ ctxdom Γ
+  end.
+
+#[global]
+Instance listctx_stale {A:Type} : Stale (listctx A) := ctxdom.
+Arguments listctx_stale /.
+
+Lemma app_one_eq_nil {A: Type}: forall (x: atom) (tau:A) Γ, ~ ([] = Γ ++ [(x, tau)]).
+Proof.
+  intros. intro H. symmetry in H. apply app_eq_nil in H. destruct H. inversion H0.
+Qed.
+
+Lemma app_one_is_cons {A: Type}: forall (x: A) l, (x::nil) ++ l = x :: l.
+Proof. simpl. reflexivity. Qed.
+
+Lemma app_list_unit_eq_unit {A: Type}: forall (x y: A) l, l ++ [x] = [y] -> x = y /\ l = [].
+Proof. intros. apply app_eq_unit in H.
+       destruct H.
+       destruct H. inversion H0. split; auto.
+       destruct H. inversion H0.
+Qed.
+
+Ltac auto_destruct_pair :=
+  repeat match goal with
+         | [a: prod _ _ |- _] => destruct a
+         end.
+
+Ltac list_app_simpl :=
+  auto_destruct_pair;
+  try auto_exfalso;
+  repeat match goal with
+    | [H: ?Γ1 ++ [(?x1, ?t1)] = ?Γ2 ++ [(?x2, ?t2)] |- _ ] => apply app_inj_tail in H; destruct H; subst
+    | [H: (?x1, ?t1) = (?x2, ?t2) |- _ ] => inversion H; subst; clear H
+    | [H: context [ ?a ++ []] |- _ ] => rewrite app_nil_r in H
+    | [ |- context [ ?a ++ []] ] => rewrite app_nil_r
+    | [H: context [ [] ++ ?a] |- _ ] => rewrite app_nil_l in H
+    | [ |- context [ [] ++ ?a] ] => rewrite app_nil_l
+    | [H: context [(_ :: _) ++ _] |- _ ] => rewrite <- app_comm_cons in H
+    | [ |- context [(_ :: _) ++ _]] => rewrite <- app_comm_cons
+    | [H: context [(_ ++ _) ++ _] |- _ ] => rewrite <- app_assoc in H
+    | [ |- context [(_ ++ _) ++ _]] => rewrite <- app_assoc
+    end; auto.
+
+Lemma ctxdom_app_union {A: Type}: forall (Γ1 Γ2: listctx A), ctxdom (Γ1 ++ Γ2) = (ctxdom Γ1) ∪ (ctxdom Γ2).
+Proof.
+  induction Γ1; simpl; intros; auto. my_set_solver.
+  auto_destruct_pair. rewrite IHΓ1. my_set_solver.
+Qed.
+
+(** Definition of non-duplicate. *)
+Inductive ok {A: Type} : (listctx A) -> Prop :=
+| ok_nil: ok nil
+| ok_cons: forall Γ (x: atom) (t: A), ok Γ -> x ∉ ctxdom Γ -> ok (Γ ++ [(x, t)]).
+
+Global Hint Constructors ok: core.
+
+Lemma ok_post_destruct {A: Type}: forall Γ (x: atom) (t: A), ok (Γ ++ [(x, t)]) <-> ok Γ /\ x ∉ ctxdom Γ.
+Proof.
+  intros. split.
+  - split; inversion H; subst; repeat list_app_simpl.
+  - intros. destruct H. constructor; auto.
+Qed.
+
+Lemma ok_pre_destruct {A: Type}: forall Γ (x: atom) (t: A), ok ((x, t) :: Γ) <-> ok Γ /\ x ∉ ctxdom Γ.
+Proof.
+  split; generalize dependent t. generalize dependent x. generalize dependent Γ.
+  - apply (rev_ind (fun Γ => forall (x: atom) (t: A), ok ((x, t) :: Γ) -> ok Γ /\ x ∉ ctxdom Γ));
+      simpl; split; intros; auto_destruct_pair; auto; try my_set_solver.
+    + rewrite app_comm_cons in H0. rewrite ok_post_destruct in H0. destruct H0.
+      specialize (H x0 t H0). destruct H.
+      constructor; auto. my_set_solver.
+    + rewrite app_comm_cons in H0. rewrite ok_post_destruct in H0. destruct H0.
+      specialize (H x0 t H0). destruct H. rewrite ctxdom_app_union. my_set_solver.
+  - apply (rev_ind (fun Γ => forall (x: atom) (t: A), ok Γ /\ x ∉ ctxdom Γ -> ok ((x, t) :: Γ)));
+      simpl; intros.
+    + destruct H. rewrite <- app_nil_l. constructor; auto.
+    + auto_destruct_pair. destruct H0.
+      rewrite ok_post_destruct in H0. destruct H0. rewrite ctxdom_app_union in H1.
+      rewrite app_comm_cons. constructor; auto. apply H; auto. split; auto. my_set_solver. my_set_solver.
+Qed.
+
+(** another ok definition *)
+Inductive ok_forward {A: Type} : (listctx A) -> Prop :=
+| ok_nil_forward: ok_forward nil
+| ok_cons_forward: forall Γ (x: atom) (t: A), ok_forward Γ -> x ∉ ctxdom Γ -> ok_forward ((x, t) :: Γ).
+
+Global Hint Constructors ok_forward: core.
+
+(** two definitions is equal *)
+Lemma ok_iff_of_ok_forward {A: Type}: forall (Γ: listctx A), ok Γ <-> ok_forward Γ.
+Proof.
+  split.
+  - induction Γ; intros; auto. destruct a. apply ok_pre_destruct in H. destruct H.
+    constructor; auto.
+  - induction Γ; intros; auto. destruct a. rewrite ok_pre_destruct.
+    inversion H; subst. split; auto.
+Qed.
+
+Lemma ok_weak_pre {A: Type}: forall (Γ1 Γ2: listctx A),
+    ok (Γ1 ++ Γ2) -> ok Γ1.
+Proof.
+  intros Γ1.
+  apply (rev_ind (fun Γ2 => ok (Γ1 ++ Γ2) -> ok Γ1)); intros.
+  - list_app_simpl.
+  - apply H. rewrite app_assoc in H0. destruct x. rewrite ok_post_destruct in H0.
+    destruct H0; auto.
+Qed.
+
+Lemma ok_weak_post {A: Type}: forall (Γ2 Γ1: listctx A),
+    ok (Γ1 ++ Γ2) -> ok Γ2.
+Proof.
+  intros Γ2. induction Γ1; intros.
+  - list_app_simpl.
+  - apply IHΓ1. rewrite ok_iff_of_ok_forward. rewrite ok_iff_of_ok_forward in H.
+    inversion H; subst. auto.
+Qed.
+
+(** ctxfind *)
+Fixpoint ctxfind {A: Type} (Γ: listctx A) (x: atom): option A :=
+  match Γ with
+  | [] => None
+  | (y, t) :: Γ => if decide (x = y) then Some t else ctxfind Γ x
+  end.
+
+Lemma ctxfind_none_iff_not_in_dom {A: Type}: forall (Γ: listctx A) x,
+    ctxfind Γ x = None <-> x ∉ ctxdom Γ.
+Proof with auto.
+  split; generalize dependent x.
+  - induction Γ; simpl; intros; try auto_destruct_pair.
+    + my_set_solver.
+    + var_dec_solver.
+      rewrite decide_True in H; auto; auto_exfalso.
+      rewrite decide_False in H; auto. apply IHΓ in H. my_set_solver.
+  - induction Γ; simpl; intros; try auto_destruct_pair; auto.
+    + var_dec_solver; auto. my_set_solver.
+Qed.
+
+Lemma ctxfind_some_implies_in_dom {A: Type}: forall (Γ: listctx A) x (a: A),
+    ctxfind Γ x = Some a -> x ∈ ctxdom Γ.
+Proof with auto.
+  induction Γ; simpl; intros; try auto_destruct_pair.
+  + auto_exfalso.
+  + repeat var_dec_solver. set_solver. apply IHΓ in H. my_set_solver.
+Qed.
+
+Ltac listctx_set_simpl' :=
+  list_app_simpl;
+  repeat match goal with
+    | [H: ctxfind _ _ = Some _ |- _ ⊆ _ ] => apply ctxfind_some_implies_in_dom in H
+    | [H: ctxfind _ _ = Some _ |- _ ∉ _ ] => apply ctxfind_some_implies_in_dom in H
+    | [H: ctxfind _ _ = Some _ |- _ ∈ _ ] => apply ctxfind_some_implies_in_dom in H
+    | [H: ctxfind _ _ = None |- _ ] => rewrite ctxfind_none_iff_not_in_dom in H
+    | [H: context [ctxdom (_ ++ _)] |- _ ] =>
+        rewrite ctxdom_app_union in H; simpl in H
+    | [|- ctxfind _ _ = None ] => rewrite ctxfind_none_iff_not_in_dom
+    | [H: ok (((?x, _) :: _) ++ [(?y, _)]) |- _ ] =>
+        rewrite <- app_comm_cons in H
+    | [H: ok ((?x, _) :: _) |- _ ] =>
+        rewrite ok_pre_destruct in H; destruct H
+    | [H: ok (_ ++ [(_, _)]) |- _ ] =>
+        rewrite ok_post_destruct in H; destruct H
+    | [H: context [ctxdom (_ ++ [(_, _)])] |- _ ] =>
+        rewrite ctxdom_app_union in H; simpl in H
+    | [|- context [ctxdom (_ ++ [(_, _)])]] =>
+        rewrite ctxdom_app_union; simpl
+    | [|- context [ctxdom (_ ++ _)]] =>
+        rewrite ctxdom_app_union; simpl
+    end.
+
+Lemma ctxfind_none_neq_hd {A: Type}: forall (Γ: listctx A) x tx a,
+    ctxfind ((x, tx):: Γ) a = None -> x <> a.
+Proof with auto.
+  intros. rewrite ctxfind_none_iff_not_in_dom in H. my_set_solver.
+Qed.
+
+Lemma ctxfind_app {A: Type}: forall Γ1 Γ2 x (T: A),
+    ok (Γ1 ++ Γ2) ->
+    ctxfind (Γ1 ++ Γ2) x = Some T <-> ctxfind Γ1 x = Some T \/ ctxfind Γ2 x = Some T.
+Proof.
+  induction Γ1; split; intros; listctx_set_simpl'.
+  - destruct H0; auto. inversion H0.
+  - destruct (Atom.atom_dec a x); subst; simpl in H0; auto.
+    + left. repeat var_dec_solver.
+    + simpl. repeat var_dec_solver. rewrite <- IHΓ1; auto.
+  - destruct H0; simpl in H0; auto.
+    + repeat var_dec_solver. rewrite IHΓ1; auto.
+    + repeat var_dec_solver. apply ctxfind_some_implies_in_dom in H0. my_set_solver.
+      rewrite IHΓ1; auto.
+Qed.
+
+Lemma ctxfind_app_exclude {A: Type}: forall (Γ1 Γ2: listctx A), ok (Γ1 ++ Γ2) -> (ctxdom Γ1) ∩ (ctxdom Γ2) = ∅.
+Proof.
+  induction Γ1; intros; simpl; listctx_set_simpl'.
+  - fast_set_solver.
+  - my_set_solver.
+Qed.
+
+Lemma ctxfind_app_weaken {A: Type}: forall Γ1 Γ2 Γ3 x (T: A),
+    ok (Γ1 ++ Γ2 ++ Γ3) ->
+    ctxfind (Γ1 ++ Γ3) x = Some T -> ctxfind (Γ1 ++ Γ2 ++ Γ3) x = Some T.
+Proof.
+  induction Γ1; simpl; intros; listctx_set_simpl'.
+  - rewrite ctxfind_app; auto.
+  - repeat var_dec_solver.
+Qed.
+
+Lemma ok_app_weaken {A: Type}: forall (Γ1 Γ2: listctx A) x (Tx :A),
+    ok (Γ1 ++ (x, Tx) :: Γ2) -> ok (Γ1 ++ Γ2).
+Proof.
+  induction Γ1; simpl; intros; listctx_set_simpl'; auto.
+  - apply IHΓ1 in H. rewrite ok_pre_destruct. split; auto. listctx_set_simpl'. my_set_solver.
+Qed.
+
+Lemma ctxfind_find_mid_eq {A: Type}: forall (Γ1 Γ3: listctx A) x (U T:A),
+    ok (Γ1 ++ (x, U) :: Γ3) ->
+    ctxfind (Γ1 ++ (x, U) :: Γ3) x = Some T -> U = T.
+Proof.
+  induction Γ1; simpl; intros; listctx_set_simpl'; auto.
+  - repeat var_dec_solver.
+  - repeat var_dec_solver. my_set_solver.
+Qed.
+
+Lemma ctxfind_find_mid_neq {A: Type}: forall (Γ1 Γ3: listctx A) x y (U T:A),
+    x <> y ->
+    ok (Γ1 ++ (x, U) :: Γ3) ->
+    ctxfind (Γ1 ++ (x, U) :: Γ3) y = Some T -> ctxfind (Γ1 ++ Γ3) y = Some T.
+Proof.
+  induction Γ1; simpl; intros; listctx_set_simpl'; auto.
+  - repeat var_dec_solver.
+  - repeat var_dec_solver. my_set_solver.
+Qed.
+
+Lemma find_mid_eq_singleton_simp {A: Type} : forall (x1 x2: atom) (τ1 τ2: A) Γ1 Γ2,
+    [(x1, τ1)] = Γ1 ++ (x2, τ2) :: Γ2 -> x1 = x2 /\ τ1 = τ2 /\ Γ1 = [] /\ Γ2 = [].
+Proof.
+  intros.
+  destruct Γ1; listctx_set_simpl'; invclear H.
+  - repeat split; auto.
+  - listctx_set_simpl'.
+Qed.
+
+
+Lemma find_mid_eq_cons_simp {A: Type} : forall (x1 x2: atom) (τ1 τ2: A) Γ1 Γ2 Γ,
+    (x1, τ1) :: Γ = Γ1 ++ (x2, τ2) :: Γ2 ->
+    (x1 = x2 /\ τ1 = τ2 /\ Γ1 = [] /\ Γ2 = Γ) \/
+      (exists Γ1', Γ = Γ1' ++ (x2, τ2) ::  Γ2 /\ Γ1 = (x1, τ1) :: Γ1').
+Proof.
+  intros.
+  destruct Γ1; invclear H.
+  - left. repeat split; auto.
+  - right. exists Γ1. repeat split; auto.
+Qed.
+
+Ltac listctx_set_simpl1 :=
+  list_app_simpl;
+  repeat (listctx_set_simpl' ||
+            (match goal with
+             | [H: context [ctxfind [] _] |- _ ] => progress simpl in H
+             | [|- context [ctxfind [] _]] => progress simpl
+             | [H1: ok (?Γ1 ++ (?x, ?U) :: ?Γ3), H: ctxfind (?Γ1 ++ (?x, ?U) :: ?Γ3) ?x = Some ?T |- _ ] => assert (U = T) as Htmp by (apply (ctxfind_find_mid_eq _ _ _ _ T) in H1; auto); subst; try clear Htmp
+             | [H: ctxfind (?Γ1 ++ (?z, _) :: ?Γ3) ?x = Some ?T
+                |- ctxfind (?Γ1 ++ ?Γ3) ?x = Some ?T ] => apply ctxfind_find_mid_neq in H; auto
+| [H: (_, _) :: _ = (_, _):: _ |- _ ] => invclear H
+            | [H: [(_, _)] = _ ++ (_, _) :: _ |- _ ] => apply find_mid_eq_singleton_simp in H; mydestr; subst
+            | [H: (_, _) :: _ = _ ++ (_, _) :: _ |- _ ] => apply find_mid_eq_cons_simp in H; destruct H; mydestr; subst
+             end)).
+
+Ltac listctx_set_simpl2 :=
+  repeat (listctx_set_simpl1 ||
+            match goal with
+            | [H: (_, _) :: _ = (_, _):: _ |- _ ] => invclear H
+            | [H: [(_, _)] = _ ++ (_, _) :: _ |- _ ] => apply find_mid_eq_singleton_simp in H; mydestr; subst
+            | [H: (_, _) :: _ = _ ++ (_, _) :: _ |- _ ] => apply find_mid_eq_cons_simp in H; destruct H; mydestr; subst
+            end).
+
+Ltac listctx_set_simpl3 :=
+  match goal with
+  | [H: _ ++ [_] = [_] |- _ ] => apply elt_eq_unit in H; mydestr; subst
+  | [H: _ ++ [_] = _ :: _ ++ [_] |- _ ] => rewrite app_comm_cons in H; listctx_set_simpl2
+  end || listctx_set_simpl2.
+
+Ltac listctx_set_simpl4 :=
+  match goal with
+  | [H: _ ++ [_] = _ ++ _ ++ [_] |- _ ] =>
+      rewrite app_assoc in H;
+      apply app_inj_tail in H; mydestr; subst; listctx_set_simpl3
+  end || listctx_set_simpl3.
+
+Ltac listctx_set_simpl := listctx_set_simpl4.
+
+Ltac listctx_set_solver1 :=
+  repeat (listctx_set_simpl;
+          match goal with
+          | [|- _ <> _] => fast_set_solver !!
+          | [|- _ = _] => fast_set_solver !!
+          | [|- _ ∉ _] => fast_set_solver !!
+          | [|- _ ∈ _] => fast_set_solver !!
+          | [|- _ ⊆ _] => fast_set_solver !!
+          | [H: ctxfind (?Γ1 ++ ?Γ3) ?x = Some ?T |- ctxfind (?Γ1 ++ ?Γ2 ++ ?Γ3) ?x = Some ?T ] => apply ctxfind_app_weaken; auto
+          | [H: ok (?Γ1 ++ _ :: ?Γ2) |- ok (?Γ1 ++ ?Γ2) ] => apply ok_app_weaken in H; exact H
+          | [H: ok (_ ++ (?x, _) :: ?Γ) |- ?x ∉ ctxdom ?Γ ] =>
+              apply ok_weak_post in H; rewrite ok_pre_destruct in H; destruct H; auto
+          | [H: ok (?a ++ ?b ++ ?c) |- ok ((?a ++ ?b) ++ ?c) ] => rewrite <- app_assoc; exact H
+          | [H: ok (?a ++ ?b ++ ?c) |- ok (?a ++ ?b ++ ?c ++ [(?x, _)]) ] =>
+              rewrite -> app_assoc; rewrite -> app_assoc; constructor
+          | [|- ok ((_, _) :: _) ] => rewrite ok_pre_destruct; split; auto
+          end); listctx_set_simpl; fast_set_solver !!.
+
+Lemma ctxfind_none_neq_tl {A: Type}: forall (Γ: listctx A) x tx a,
+    ctxfind ((x, tx):: Γ) a = None -> ctxfind Γ a = None.
+Proof. intros; listctx_set_solver1. Qed.
+
+Lemma ctxfind_weak_pre {A: Type}: forall (Γ1 Γ2 : listctx A) a,
+    ctxfind (Γ1 ++ Γ2) a = None ->
+    ctxfind Γ1 a = None.
+Proof. intros; listctx_set_solver1. Qed.
+
+Lemma ctxfind_weak_post {A: Type}: forall (Γ1  Γ2: listctx A) a,
+    ctxfind (Γ1 ++ Γ2) a = None ->
+    ctxfind Γ2 a = None.
+Proof. intros; listctx_set_solver1. Qed.
+
+Lemma ctxfind_weak_unit {A: Type}: forall x (tau_x: A) a,
+    ctxfind ((x, tau_x)::nil) a = None -> a <> x.
+Proof. intros; listctx_set_solver1. Qed.
+
+Lemma l_find_implies_in {A:Type}: forall (ctx: listctx A) (x: atom) (t: A),
+      ctxfind ctx x = Some t -> In (x, t) ctx.
+Proof.
+  induction ctx; simpl; intros; listctx_set_simpl.
+  var_dec_solver.
+  + left. var_dec_solver; auto_eq_post.
+  + right. var_dec_solver.
+Qed.
+
+Lemma ctxfind_some_spec_aux {A:Type}: forall (ctx: list (prod atom A)) (name: atom) (tau: A),
+  ctxfind ctx name = Some tau ->
+  (exists ctx1 ctx2,
+      ctx = ctx1 ++ ((name, tau)::nil) ++ ctx2
+  ).
+Proof with auto.
+  intros.
+  apply l_find_implies_in in H. apply in_split in H. destruct H as (G1 & G2 & HG12).
+  exists G1, G2. subst. split...
+Qed.
+
+Lemma ok_first_not_equal_hd {A:Type}: forall (Γ: list (prod atom A)) (x y: atom) (a b: A),
+    ok ((x, a) :: Γ ++ [(y, b)]) -> x <> y.
+Proof.
+  intros. listctx_set_simpl. listctx_set_solver1.
+Qed.
+
+Ltac auto_exfalso_ok :=
+  try match goal with
+    | [H: ctxfind [] _ = Some _ |- _ ] => inversion H
+    | [H: ok (((?x, _) :: ?Γ) ++ [(?x, _)]) |- _ ] =>
+        rewrite <- app_comm_cons in H; apply ok_first_not_equal_hd in H; exfalso; auto
+    | [H: ok ((?x, _) :: ?Γ ++ [(?x, _)]) |- _ ] =>
+        apply ok_first_not_equal_hd in H; exfalso; auto
+    end;
+  auto_exfalso.
+
+Ltac listctx_set_solver2 :=
+  repeat match goal with
+    | [H: ok ?Γ |- ok [(?x, _); (?y, _)]] => rewrite <- app_one_is_cons; constructor; auto
+    | [H: ok ?Γ |- ok (?Γ ++ [(?x, _); (?y, _)])] => rewrite <- app_one_is_cons; rewrite app_assoc; constructor; auto
+    | [H: ok ?Γ |- ok (?Γ ++ [(?x, _)])] => econstructor; eauto
+    end; auto;
+  (auto_exfalso_ok || listctx_set_solver1).
+
+Lemma ctxfind_last_eq {A:Type}: forall (ctx: list (prod atom A)) name tau,
+    ok (ctx ++ [(name, tau)]) ->
+    ctxfind (ctx ++ [(name, tau)]) name = Some tau.
+Proof with eauto.
+  induction ctx; intros; listctx_set_simpl.
+  - repeat var_dec_solver.
+  - simpl. rewrite decide_False. apply IHctx. constructor; auto. my_set_solver.
+Qed.
+
+Ltac var_dec_solver_exfalso :=
+  var_dec_solver;
+  try auto_exfalso_ok.
+
+Lemma ctxfind_last_neq_none {A:Type}: forall (ctx: list (prod atom A)) name tau a,
+    name <> a ->
+    ctxfind (ctx ++ [(name, tau)]) a = None <->
+      ctxfind ctx a = None.
+Proof. split; intros; listctx_set_solver2. Qed.
+
+Lemma ctxfind_last_neq {A:Type}: forall (ctx: list (prod atom A)) name tau a tau_a,
+    ok (ctx ++ [(name, tau)]) ->
+    name <> a ->
+    ctxfind (ctx ++ [(name, tau)]) a = Some tau_a <->
+      ctxfind ctx a = Some tau_a.
+Proof with eauto.
+  intros. induction ctx...
+  - simpl. split; intros; repeat var_dec_solver_exfalso.
+  - try auto_destruct_pair.
+    listctx_set_simpl.
+    simpl. split; intros; repeat var_dec_solver_exfalso.
+    apply IHctx in H3; auto. rewrite IHctx; auto.
+Qed.
+
+Lemma ctxfind_some_spec {A:Type}: forall (ctx: list (prod atom A)) (name: atom) (tau: A),
+    ok ctx ->
+    ctxfind ctx name = Some tau ->
+    (exists ctx1 ctx2,
+        ctx = ctx1 ++ [(name, tau)] ++ ctx2 /\ ctxfind ctx2 name = None
+    ).
+Proof.
+  intros.
+  apply ctxfind_some_spec_aux in H0.
+  destruct H0 as (Γ1 & Γ2 & Happ). exists Γ1, Γ2. split; auto.
+  rewrite Happ in H. listctx_set_solver2.
+Qed.
+
+Lemma find_none_append {A: Type}: forall Γ a (tau_x: A) x,
+    ctxfind Γ a = None ->
+    x <> a ->
+    ctxfind (Γ ++ ((x,tau_x)::nil)) a = None.
+Proof with eauto.
+  intros. listctx_set_solver2.
+Qed.
+
+Ltac listctx_set_solver3 :=
+  simpl;
+  repeat match goal with
+    | [H: ok (_ ++ ?Γ) |- ok ?Γ] => apply ok_weak_post in H; auto
+    | [H: ok (?Γ ++ _) |- ok ?Γ] => apply ok_weak_pre in H; auto
+    | [|- _ ∉ _ ] => listctx_set_solver2
+    | [ |- ok [(_, _); (?x, ?T); (_, _)]] => rewrite <- app_one_is_cons; rewrite <- (app_one_is_cons (x, T)); rewrite app_assoc; constructor; auto
+    | [H: ok ?Γ |- ok [(_, _); (?x, ?T); (_, _)]] =>
+        rewrite <- app_one_is_cons;
+        rewrite app_assoc; rewrite <- (app_one_is_cons (x, T));
+        rewrite app_assoc; constructor; auto
+    | [H: ok ?Γ |- ok [(?x, _); (?y, _)]] => rewrite <- app_one_is_cons; constructor; auto
+    | [|- ok [(_, _)]] => rewrite <- app_nil_l; constructor; auto
+    | [|- ok (?Γ ++ [(?x, _)])] => econstructor; eauto
+    | [H: ok ?Γ |- ok (?Γ ++ [(?x, _); (?y, _)])] => rewrite <- app_one_is_cons; rewrite app_assoc; constructor; auto
+    | [H: ok ?Γ |- ok (?Γ ++ [(_, _); (?x, ?T); (_, _)])] =>
+        rewrite <- app_one_is_cons;
+        rewrite app_assoc; rewrite <- (app_one_is_cons (x, T));
+        rewrite app_assoc; constructor; auto
+    end; auto;
+  listctx_set_solver2.
+
+Lemma ok_single {A: Type}: forall (x: atom) (T: A), ok [(x, T)].
+Proof.
+  intros.
+  rewrite ok_pre_destruct; split; auto; fast_set_solver.
+Qed.
+
+Ltac listctx_set_solver4 :=
+  match goal with
+  | [|- ok [(_, _)]] => apply ok_single
+  end || listctx_set_solver3.
+
+Lemma ctxfind_in {A: Type}: forall Γv1 (x: atom) (u: A) Γv2,
+    ok (Γv1 ++ (x, u) :: Γv2) ->
+    ctxfind (Γv1 ++ (x, u) :: Γv2) x = Some u.
+Proof.
+  induction Γv1; simpl; intros; mydestr; auto.
+  - repeat var_dec_solver.
+  - repeat var_dec_solver; listctx_set_solver4.
+Qed.
+
+Lemma ok_mid_insert {A: Type} : forall Γ1 (x: atom) (T: A) Γ2,
+    (x ∉ ctxdom Γ1 ∪ ctxdom Γ2 /\ ok (Γ1 ++ Γ2)) <-> ok (Γ1 ++ (x, T) :: Γ2).
+Proof.
+  induction Γ1; split; simpl; intros; mydestr; repeat split; auto; try listctx_set_solver4.
+  - rewrite ok_pre_destruct. split.
+    + apply IHΓ1; repeat split; listctx_set_solver4.
+    + listctx_set_solver4.
+  - rewrite ok_pre_destruct in H; mydestr. rewrite <- IHΓ1 in H; mydestr. listctx_set_solver4.
+Qed.
+
+Lemma ok_app_swap {A: Type} : forall (Γ1: listctx A) Γ2, ok (Γ1 ++ Γ2) <-> ok (Γ2 ++ Γ1).
+Proof.
+  induction Γ1; split; simpl; intros; mydestr; try listctx_set_solver4.
+  - rewrite ok_pre_destruct in H; mydestr. rewrite IHΓ1 in H.
+    rewrite <- ok_mid_insert; split; listctx_set_solver4.
+  - rewrite <- ok_mid_insert in H; mydestr. rewrite <- IHΓ1 in H0.
+    rewrite ok_pre_destruct; split; auto; listctx_set_solver4.
+Qed.
+
+Lemma ok_app_swap3 {A: Type} : forall (Γ1: listctx A) Γ2 Γ3, ok (Γ1 ++ Γ2 ++ Γ3) <-> ok (Γ2 ++ Γ1 ++ Γ3).
+Proof.
+  induction Γ1; split; simpl; intros; mydestr; try listctx_set_solver4.
+  - rewrite ok_pre_destruct in H; mydestr. rewrite IHΓ1 in H.
+    rewrite <- ok_mid_insert; split; listctx_set_solver4.
+  - rewrite <- ok_mid_insert in H; mydestr. rewrite <- IHΓ1 in H0.
+    rewrite ok_pre_destruct; split; auto; listctx_set_solver4.
+Qed.
+
+Ltac listctx_set_solver5 :=
+  match goal with
+  | [H: ok (?a ++ ?b) |- ok (?b ++ ?a)] => rewrite ok_app_swap; auto
+  | [H: ok (?a ++ ?b ++ ?c) |- ok (?b ++ ?a ++ ?c)] => rewrite ok_app_swap3; auto
+  | [H: ok (?Γ1 ++ ?Γ2 ++ ?Γ3) |- ok (?Γ1 ++ ?Γ3)] =>
+         rewrite ok_app_swap3 in H; listctx_set_solver4
+  end || listctx_set_solver4.
+
+Ltac listctx_set_solver := listctx_set_solver5.
+
+Lemma ok_find_same {A: Type}: forall (a: atom) (τ1 τ2: A) Γ1 Γ2 Γ1' Γ2',
+    ok (Γ1 ++ ((a, τ1) :: Γ2)) -> (Γ1 ++ ((a, τ1) :: Γ2)) = (Γ1' ++ (a, τ2) :: Γ2') ->
+    Γ1 = Γ1' /\ τ1 = τ2 /\ Γ2 = Γ2'.
+Proof.
+  intros a τ1 τ2.
+  induction Γ1; intros; listctx_set_simpl2.
+  apply IHΓ1 in H0; auto. mydestr; subst.
+  repeat split; auto.
+Qed.
+
+Lemma ok_find_neq_head {A: Type}: forall (x a: atom) (τ_x τ_a: A) Γ1' Γ2 Γ2',
+    x <> a ->
+    ok ((x, τ_x) :: Γ2) -> ((x, τ_x) :: Γ2) = (Γ1' ++ (a, τ_a) :: Γ2') ->
+    (exists Γ1'', Γ1' = (x, τ_x) :: Γ1'' /\ Γ2 = (Γ1'' ++ (a, τ_a) :: Γ2')).
+Proof.
+  intros x a τ_x τ_a Γ1'.
+  induction Γ1'; intros; listctx_set_simpl2.
+  exists Γ1'. split; auto.
+Qed.
