formalization/RefinementType.v
@@ -1,0 +1,551 @@
+From stdpp Require Import mapset.
+From stdpp Require Import natmap.
+From CT Require Import CoreLangClass.
+From CT Require Import OperationalSemantics.
+From CT Require Import BasicTypingClass.
+From CT Require Import QualifierClass.
+From CT Require Import ListCtx.
+
+Import Atom.
+Import CoreLang.
+Import Tactics.
+Import NamelessTactics.
+Import OperationalSemantics.
+Import BasicTyping.
+Import Qualifier.
+Import ListCtx.
+Import List.
+
+Inductive rty : Type :=
+| overrty (b: base_ty) (ϕ: qualifier)
+| underrty (b: base_ty) (ϕ: qualifier)
+| arrrty (ρ: rty) (τ: rty).
+
+Global Hint Constructors rty: core.
+
+Notation "'{:' B '|' ϕ '}'" := (overrty B ϕ) (at level 5, format "{: B | ϕ }", B constr, ϕ constr).
+Notation "'[:' B '|' ϕ ']'" := (underrty B ϕ) (at level 5, format "[: B | ϕ ]", B constr, ϕ constr).
+Notation "ρ '⇨' τ " :=
+ (arrrty ρ τ) (at level 80, format "ρ ⇨ τ", right associativity, ρ constr, τ constr).
+
+(** Type erasure (Fig. 5) *)
+
+Fixpoint rty_erase ρ : ty :=
+  match ρ with
+  | {: B | _} => B
+  | [: B | _] => B
+  | ρ ⇨ τ => (rty_erase ρ) ⤍ (rty_erase τ)
+  end.
+
+Definition ctx_erase (Γ: listctx rty) :=
+  ⋃ ((List.map (fun e => {[e.1 := rty_erase e.2]}) Γ): list (amap ty)).
+
+Class Erase A B := erase : A -> B.
+#[global] Instance rty_erase_ : Erase rty ty := rty_erase.
+#[global] Instance ctx_erase_ : Erase (listctx rty) (amap ty) := ctx_erase.
+
+Notation " '⌊' ty '⌋' " := (erase ty) (at level 5, format "⌊ ty ⌋", ty constr).
+
+(** * Naming related definitions *)
+
+(** free variables *)
+Fixpoint rty_fv ρ : aset :=
+  match ρ with
+  | {: _ | ϕ } => qualifier_fv ϕ
+  | [: _ | ϕ ] => qualifier_fv ϕ
+  | ρ ⇨ τ => rty_fv ρ ∪ rty_fv τ
+  end.
+
+#[global]
+  Instance rty_stale : @Stale aset rty := rty_fv.
+Arguments rty_stale /.
+
+Fixpoint rty_open (k: nat) (s: value) (ρ: rty) : rty :=
+  match ρ with
+  | {: B | ϕ } => {: B | qualifier_open (S k) s ϕ }
+  | [: B | ϕ ] => [: B | qualifier_open (S k) s ϕ ]
+  | ρ ⇨ τ => (rty_open k s ρ) ⇨ (rty_open (S k) s τ)
+  end.
+
+(** never use *)
+Definition _close_rty (x: atom) (k: nat) (ρ: rty) : rty := ρ.
+
+Fixpoint rty_subst (k: atom) (s: value) (ρ: rty) : rty :=
+  match ρ with
+  | {: B | ϕ } => {: B | qualifier_subst k s ϕ }
+  | [: B | ϕ ] => [: B | qualifier_subst k s ϕ ]
+  | ρ ⇨ τ => (rty_subst k s ρ) ⇨ (rty_subst k s τ)
+  end.
+
+Inductive lc_rty : rty -> Prop :=
+| lc_rty_over_base: forall B ϕ (L : aset),
+    (forall x : atom, x ∉ L -> lc_qualifier (qualifier_open 0 x ϕ)) ->
+    lc_rty {: B | ϕ }
+| lc_rty_under_base: forall B ϕ (L : aset),
+    (forall x : atom, x ∉ L -> lc_qualifier (qualifier_open 0 x ϕ)) ->
+    lc_rty [: B | ϕ ]
+| lc_rty_arr: forall ρ τ (L : aset),
+    lc_rty ρ ->
+    (forall x : atom, x ∉ L -> lc_rty (rty_open 0 x τ)) ->
+    lc_rty (ρ ⇨ τ).
+
+Definition body_rty (e: rty) := exists (L: aset), forall (x: atom), x ∉ L -> lc_rty (rty_open 0 (vfvar x) e).
+
+#[export] Instance rty_substable : Substable rty :=
+  {
+    substitute := rty_subst;
+    fv := rty_fv;
+  }.
+
+#[export] Instance rty_ast : Ast rty :=
+  {
+    open := rty_open;
+    lc := lc_rty;
+    body := body_rty;
+    close := _close_rty;
+  }.
+
+(* Notation "'{' k '~>' s '}' e" := (rty_open k s e) (at level 20, k constr). *)
+(* Notation "'{' k '~>' s '}' e" := (am_open k s e) (at level 20, k constr). *)
+(* Notation "'{' k '~>' s '}' e" := (rty_open k s e) (at level 20, k constr). *)
+(* Notation "e '^p^' s" := (rty_open 0 s e) (at level 20). *)
+(* Notation "e '^a^' s" := (am_open 0 s e) (at level 20). *)
+(* Notation "e '^h^' s" := (rty_open 0 s e) (at level 20). *)
+
+(* Notation "'{' x ':=' s '}'" := (rty_subst x s) (at level 20, format "{ x := s }", x constr). *)
+(* Notation "'{' x ':=' s '}a'" := (am_subst x s) (at level 20, format "{ x := s }a", x constr). *)
+(* Notation "'{' x ':=' s '}h'" := (rty_subst x s) (at level 20, format "{ x := s }h", x constr). *)
+(** Closed under free variable set *)
+Inductive closed_rty (d : aset) (ρ: rty): Prop :=
+| closed_rty_: lc_rty ρ -> rty_fv ρ ⊆ d -> closed_rty d ρ.
+
+(** Well-formedness of type context. All terms and types are alpha-converted to
+  have unique names. *)
+Inductive ok_ctx: listctx rty -> Prop :=
+| ok_ctx_nil: ok_ctx []
+| ok_ctx_cons: forall (Γ: listctx rty)(x: atom) (ρ: rty),
+    ok_ctx Γ ->
+    closed_rty (ctxdom Γ) ρ ->
+    x ∉ ctxdom Γ ->
+    ok_ctx (Γ ++ [(x, ρ)]).
+
+Lemma ok_ctx_ok: forall Γ, ok_ctx Γ -> ok Γ.
+Proof.
+  induction 1; eauto.
+Qed.
+
+(** Shorthands *)
+Definition mk_eq_constant c := [: ty_of_const c | b0:c= c ].
+Definition mk_bot ty := [: ty | mk_q_under_bot ].
+Definition mk_top ty := [: ty | mk_q_under_top ].
+Definition mk_eq_var ty (x: atom) := [: ty | b0:x= x ].
+
+(** * Naming properties of refinement type syntax *)
+
+
+Lemma rty_erase_open_eq (ρ: rty) k s : erase ρ = erase ({k ~> s} ρ).
+Proof.
+  generalize dependent k.
+  unfold open. unfold erase.
+  induction ρ; simpl in *; eauto.
+  intros. rewrite <- IHρ1. rewrite <- IHρ2. auto.
+Qed.
+
+Lemma rty_erase_subst_eq (ρ: rty) x s : erase ρ = erase ({x := s} ρ).
+Proof.
+  unfold substitute. unfold erase.
+  induction ρ; simpl in *; eauto.
+  rewrite <- IHρ1. rewrite <- IHρ2. auto.
+Qed.
+
+Lemma ctx_erase_lookup Γ x ρ :
+  ctxfind Γ x = Some ρ ->
+  ⌊Γ⌋ !! x = Some ⌊ρ⌋.
+Proof.
+  induction Γ; simpl; intros; try easy.
+  destruct a. case_decide. simplify_eq.
+  cbn. simplify_map_eq. reflexivity.
+  simp_hyps.
+  cbn. rewrite insert_empty. rewrite <- insert_union_singleton_l.
+  simplify_map_eq. reflexivity.
+Qed.
+
+Lemma ctx_erase_app Γ Γ':
+  ⌊Γ ++ Γ'⌋ = ⌊Γ⌋ ∪ ⌊Γ'⌋.
+Proof.
+  unfold erase.
+  induction Γ; simpl.
+  - cbn. by rewrite map_empty_union.
+  - destruct a. unfold ctx_erase_ in *. cbn. unfold ctx_erase in *. rewrite IHΓ.
+    by rewrite map_union_assoc.
+Qed.
+
+Lemma ctx_erase_dom Γ :
+  dom ⌊Γ⌋ ≡ ctxdom Γ.
+Proof.
+  induction Γ; simpl.
+  - cbn. apply dom_empty.
+  - destruct a. cbn in *.
+    rewrite insert_empty.
+    setoid_rewrite dom_union.
+    rewrite dom_singleton.
+    f_equiv. eauto.
+Qed.
+
+Lemma ctx_erase_app_r Γ x ρ :
+  x # Γ ->
+  ⌊Γ ++ [(x, ρ)]⌋ = <[x:=⌊ρ⌋]> ⌊Γ⌋.
+Proof.
+  intros H.
+  rewrite ctx_erase_app.
+  cbn. rewrite map_union_empty. rewrite insert_empty.
+  rewrite <- insert_union_singleton_r. auto.
+  simpl in H. rewrite <- ctx_erase_dom in H.
+  by apply not_elem_of_dom.
+Qed.
+
+Lemma subst_commute_am : forall x u_x y u_y a,
+    x <> y -> x ∉ fv_value u_y -> y ∉ fv_value u_x ->
+    {x := u_x }a ({y := u_y }a a) = {y := u_y }a ({x := u_x }a a).
+Proof.
+  intros.
+  induction a; simpl; eauto; f_equal; eauto using subst_commute_qualifier.
+Qed.
+
+Lemma subst_commute_rty : forall x u_x y u_y ρ,
+    x <> y -> x ∉ fv_value u_y -> y ∉ fv_value u_x ->
+    {x := u_x } ({y := u_y } ρ) = {y := u_y } ({x := u_x } ρ)
+with subst_commute_rty : forall x u_x y u_y τ,
+    x <> y -> x ∉ fv_value u_y -> y ∉ fv_value u_x ->
+    {x := u_x }h ({y := u_y }h τ) = {y := u_y }h ({x := u_x }h τ).
+Proof.
+  destruct ρ; simpl; intros; f_equal;
+    eauto using subst_commute_qualifier, subst_commute_am.
+  destruct τ; simpl; intros; f_equal;
+    eauto using subst_commute_qualifier, subst_commute_am.
+Qed.
+
+Lemma subst_fresh_am: forall (a: am) (x:atom) (u: value),
+    x # a -> {x := u}a a = a.
+Proof.
+  intros. induction a; simpl in *; eauto; repeat f_equal;
+    eauto using subst_fresh_qualifier;
+    auto_apply; try my_set_solver.
+Qed.
+
+Lemma subst_fresh_rty: forall (ρ: rty) (x:atom) (u: value),
+    x # ρ -> {x := u} ρ = ρ
+with subst_fresh_rty: forall (τ: rty) (x:atom) (u: value),
+    x # τ -> {x := u}h τ = τ.
+Proof.
+  destruct ρ; simpl; intros; f_equal; eauto using subst_fresh_qualifier;
+    auto_apply; my_set_solver.
+  destruct τ; simpl; intros; f_equal;
+    solve [ auto_apply; my_set_solver
+          | apply subst_fresh_am; my_set_solver ].
+Qed.
+
+Lemma open_fv_am (a : am) (v : value) k :
+  am_fv ({k ~> v} a) ⊆ am_fv a ∪ fv_value v.
+Proof.
+  induction a; simpl; eauto using open_fv_qualifier;
+    repeat my_set_solver.
+Qed.
+
+Lemma open_fv_am' (a : am) (v : value) k :
+  am_fv a ⊆ am_fv ({k ~> v} a).
+Proof.
+  induction a; simpl; eauto using open_fv_qualifier';
+    my_set_solver.
+Qed.
+
+Lemma open_fv_rty (ρ : rty) (v : value) k :
+  rty_fv ({k ~> v} ρ) ⊆ rty_fv ρ ∪ fv_value v
+with open_fv_rty (τ : rty) (v : value) k :
+  rty_fv ({k ~> v} τ) ⊆ rty_fv τ ∪ fv_value v.
+Proof.
+  all: revert k.
+  destruct ρ; simpl; intros; eauto using open_fv_qualifier.
+  etrans. apply union_mono; eauto. my_set_solver.
+  destruct τ; simpl; intros.
+  etrans. repeat apply union_mono; eauto using open_fv_am. my_set_solver.
+  etrans. repeat apply union_mono; eauto. my_set_solver.
+Qed.
+
+Lemma open_fv_rty' (ρ : rty) (v : value) k :
+  rty_fv ρ ⊆ rty_fv ({k ~> v} ρ)
+with open_fv_rty' (τ : rty) (v : value) k :
+  rty_fv τ ⊆ rty_fv ({k ~> v} τ).
+Proof.
+  all: revert k.
+  destruct ρ; simpl; intros; eauto using open_fv_qualifier';
+    repeat apply union_mono; eauto.
+  destruct τ; simpl; intros;
+    repeat apply union_mono; eauto using open_fv_am'.
+Qed.
+
+Lemma open_subst_same_am: forall x y (a : am) k,
+    x # a ->
+    {x := y }a ({k ~> x} a) = {k ~> y} a.
+Proof.
+  induction a; cbn; intros; eauto.
+  f_equal. eauto using open_subst_same_qualifier.
+  all:
+  repeat
+    match goal with
+    | H : forall k, _ # _ -> _ =_ |- _ => rewrite H by my_set_solver; eauto
+    end.
+Qed.
+
+Lemma not_in_union_list {A C} `{SemiSet A C} (x : A) (ss : list C):
+  x ∉ ⋃ ss ->
+  forall s, In s ss -> x ∉ s.
+Proof.
+  induction ss; cbn; intros; eauto.
+  qsimpl.
+Qed.
+
+Lemma open_subst_same_rty: forall x y (ρ : rty) k,
+    x # ρ ->
+    {x := y } ({k ~> x} ρ) = {k ~> y} ρ
+with open_subst_same_rty: forall x y (τ : rty) k,
+    x # τ ->
+    {x := y }h ({k ~> x} τ) = {k ~> y} τ.
+Proof.
+  destruct ρ; simpl; intros; f_equal; eauto using open_subst_same_qualifier;
+    auto_apply; my_set_solver.
+  destruct τ; simpl; intros; f_equal;
+    solve [ auto_apply; my_set_solver
+          | apply open_subst_same_am; my_set_solver ].
+Qed.
+
+Lemma subst_open_am: forall (a: am) (x:atom) (u: value) (w: value) (k: nat),
+    lc w -> {x := w}a ({k ~> u} a) = ({k ~> {x := w}v u} ({x := w}a a)).
+Proof.
+  induction a; cbn; intros; eauto.
+  f_equal. eauto using subst_open_qualifier.
+  all:
+  repeat
+    match goal with
+    | H : context [lc _ -> _] |- _ => rewrite H by my_set_solver; eauto
+    end.
+Qed.
+
+Lemma subst_open_rty: forall (ρ: rty) (x:atom) (u: value) (w: value) (k: nat),
+    lc w -> {x := w} ({k ~> u} ρ) = ({k ~> {x := w}v u} ({x := w} ρ))
+with subst_open_rty: forall (τ: rty) (x:atom) (u: value) (w: value) (k: nat),
+    lc w -> {x := w}h ({k ~> u} τ) = ({k ~> {x := w}v u} ({x := w}h τ)).
+Proof.
+  destruct ρ; simpl; intros; f_equal; eauto using subst_open_qualifier.
+  destruct τ; simpl; intros; f_equal; eauto using subst_open_am.
+Qed.
+
+Lemma subst_open_rty_closed:
+  ∀ (ρ : rty) (x : atom) (u w : value) (k : nat),
+    closed_value u ->
+    lc w → {x := w } ({k ~> u} ρ) = {k ~> u} ({x := w } ρ).
+Proof.
+  intros. rewrite subst_open_rty; auto.
+  rewrite (subst_fresh_value); eauto. set_solver.
+Qed.
+
+Lemma subst_open_am_closed:
+  ∀ (a : am) (x : atom) (u w : value) (k : nat),
+    closed_value u ->
+    lc w → {x := w }a ({k ~> u} a) = {k ~> u} ({x := w }a a).
+Proof.
+  intros. rewrite subst_open_am; auto.
+  rewrite (subst_fresh_value); eauto. set_solver.
+Qed.
+
+Lemma subst_open_rty_closed:
+  ∀ (τ : rty) (x : atom) (u w : value) (k : nat),
+    closed_value u ->
+    lc w → {x := w }h ({k ~> u} τ) = {k ~> u} ({x := w }h τ).
+Proof.
+  intros. rewrite subst_open_rty; auto.
+  rewrite (subst_fresh_value); eauto. set_solver.
+Qed.
+
+Lemma subst_open_var_am: forall x y (u: value) (a: am) (k: nat),
+    x <> y -> lc u -> {x := u}a ({k ~> y} a) = ({k ~> y} ({x := u}a a)).
+Proof.
+  intros.
+  rewrite subst_open_am; auto. simpl. rewrite decide_False; auto.
+Qed.
+
+Lemma subst_open_var_rty: forall x y (u: value) (ρ: rty) (k: nat),
+    x <> y -> lc u -> {x := u} ({k ~> y} ρ) = ({k ~> y} ({x := u} ρ)).
+Proof.
+  intros.
+  rewrite subst_open_rty; auto. simpl. rewrite decide_False; auto.
+Qed.
+
+Lemma subst_open_var_rty: forall x y (u: value) (τ: rty) (k: nat),
+    x <> y -> lc u -> {x := u}h ({k ~> y} τ) = ({k ~> y} ({x := u}h τ)).
+Proof.
+  intros.
+  rewrite subst_open_rty; auto. simpl. rewrite decide_False; auto.
+Qed.
+
+Lemma subst_lc_am : forall x (u: value) (a: am),
+    lc_am a -> lc u -> lc_am ({x := u}a a).
+Proof.
+  induction 1; intros Hu; eauto using lc_am.
+  econstructor.
+  auto_exists_L_intros.
+  specialize_with x0.
+  specialize_with y.
+  rewrite <- !subst_open_var_qualifier by (eauto; my_set_solver).
+  eauto using subst_lc_qualifier.
+Qed.
+
+Lemma subst_lc_rty : forall x (u: value) (ρ: rty),
+    lc_rty ρ -> lc u -> lc_rty ({x := u} ρ)
+with subst_lc_rty : forall x (u: value) (τ: rty),
+    lc_rty τ -> lc u -> lc_rty ({x := u}h τ).
+Proof.
+  all: destruct 1; intros; simpl; econstructor; eauto using subst_lc_am;
+    instantiate_atom_listctx.
+  - rewrite <- subst_open_var_qualifier by (eauto; my_set_solver);
+      eauto using subst_lc_qualifier.
+  - rewrite <- subst_open_var_rty by (eauto; my_set_solver); eauto.
+  - rewrite <- subst_open_var_rty by (eauto; my_set_solver); eauto.
+Qed.
+
+Lemma fv_of_subst_am_closed:
+  forall x (u : value) (a: am),
+    closed_value u ->
+    am_fv ({x := u }a a) = (am_fv a ∖ {[x]}).
+Proof.
+  induction a; simpl; eauto using fv_of_subst_qualifier_closed; my_set_solver.
+Qed.
+
+Lemma fv_of_subst_rty_closed:
+  forall x (u : value) (ρ: rty),
+    closed_value u ->
+    rty_fv ({x := u } ρ) = (rty_fv ρ ∖ {[x]})
+with fv_of_subst_rty_closed:
+  forall x (u : value) (τ: rty),
+    closed_value u ->
+    rty_fv ({x := u }h τ) = (rty_fv τ ∖ {[x]}).
+Proof.
+  destruct ρ; simpl; intros; eauto using fv_of_subst_qualifier_closed.
+  rewrite !fv_of_subst_rty_closed, !fv_of_subst_rty_closed by eauto.
+  my_set_solver.
+  destruct τ; simpl; intros.
+  rewrite !fv_of_subst_am_closed, !fv_of_subst_rty_closed by eauto.
+  my_set_solver.
+  rewrite !fv_of_subst_rty_closed by eauto.
+  my_set_solver.
+Qed.
+
+Lemma open_not_in_eq_am (x : atom) (a : am) k :
+  x # {k ~> x} a ->
+  forall e, a = {k ~> e} a.
+Proof.
+  induction a; simpl; intros; eauto.
+  f_equal. eapply open_not_in_eq_qualifier. my_set_solver.
+  all: f_equal; auto_apply; my_set_solver.
+Qed.
+
+Lemma open_not_in_eq_rty (x : atom) (ρ : rty) k :
+  x # {k ~> x} ρ ->
+  forall e, ρ = {k ~> e} ρ
+with open_not_in_eq_rty (x : atom) (τ : rty) k :
+  x # {k ~> x} τ ->
+  forall e, τ = {k ~> e} τ.
+Proof.
+  all: revert k; specialize (open_not_in_eq_rty x); specialize (open_not_in_eq_rty x).
+  destruct ρ; simpl; intros; f_equal; eauto using open_not_in_eq_qualifier;
+    auto_apply; my_set_solver.
+  destruct τ; simpl; intros; f_equal;
+    solve [ auto_apply; my_set_solver
+          | apply (open_not_in_eq_am x); my_set_solver ].
+Qed.
+
+Lemma subst_intro_rty: forall (ρ: rty) (x:atom) (w: value) (k: nat),
+    x # ρ ->
+    lc w -> {x := w} ({k ~> x} ρ) = ({k ~> w} ρ).
+Proof.
+  intros.
+  specialize (subst_open_rty ρ x x w k) as J.
+  simpl in J. rewrite decide_True in J; auto.
+  rewrite J; auto. rewrite subst_fresh_rty; auto.
+Qed.
+
+Lemma lc_subst_am:
+  forall x (u: value) (a: am), lc_am ({x := u}a a) -> lc u -> lc_am a.
+Proof.
+  intros.
+  remember (({x:=u}a) a).
+  generalize dependent a.
+  induction H; intros;
+      match goal with
+      | H : _ = {_:=_}a ?a |- _ => destruct a; simpl in *; simplify_eq
+      end; eauto using lc_am.
+  econstructor.
+  auto_exists_L_intros. specialize_with x0. specialize_with y.
+  rewrite <- !subst_open_var_qualifier in H by (eauto; my_set_solver).
+  eauto using lc_subst_qualifier.
+Qed.
+
+Lemma lc_subst_rty: forall x (u: value) (ρ: rty), lc_rty ({x := u} ρ) -> lc u -> lc_rty ρ
+with lc_subst_rty: forall x (u: value) (τ: rty), lc_rty ({x := u}h τ) -> lc u -> lc_rty τ.
+Proof.
+  intros.
+  remember (({x:=u}) ρ).
+  generalize dependent ρ.
+  destruct H; intros ρ' **; destruct ρ'; simpl in *; simplify_eq;
+    econstructor; eauto;
+    instantiate_atom_listctx.
+  rewrite <- subst_open_var_qualifier in * by (eauto; my_set_solver);
+    eauto using lc_subst_qualifier.
+  rewrite <- subst_open_var_rty in * by (eauto; my_set_solver); eauto.
+  rewrite <- subst_open_var_rty in * by (eauto; my_set_solver); eauto.
+
+  intros.
+  remember (({x:=u}h) τ).
+  generalize dependent τ.
+  destruct H; intros τ' **; destruct τ'; simpl in *; simplify_eq;
+    econstructor; eauto using lc_subst_am.
+Qed.
+
+Lemma open_am_idemp: forall u (v: value) (a: am) (k: nat),
+    lc v ->
+    {k ~> u} ({k ~> v} a) = ({k ~> v} a).
+Proof.
+  induction a; intros; simpl; f_equal; eauto using open_qualifier_idemp.
+Qed.
+
+Lemma open_rty_idemp: forall u (v: value) (ρ: rty) (k: nat),
+    lc v ->
+    {k ~> u} ({k ~> v} ρ) = {k ~> v} ρ
+with open_rty_idemp: forall u (v: value)  (τ: rty) (k: nat),
+    lc v ->
+    {k ~> u} ({k ~> v} τ) = {k ~> v} τ.
+Proof.
+  destruct ρ; intros; simpl; f_equal; eauto using open_qualifier_idemp.
+  destruct τ; intros; simpl; f_equal; eauto using open_am_idemp.
+Qed.
+
+Lemma closed_rty_subseteq_proper s1 s2 ρ :
+  closed_rty s1 ρ ->
+  s1 ⊆ s2 ->
+  closed_rty s2 ρ.
+Proof.
+  intros. sinvert H. split. eauto.
+  my_set_solver.
+Qed.
+
+Lemma closed_rty_hoare_congr d ρ a b :
+  closed_rty d ρ ->
+  closed_am d a ->
+  closed_am d b ->
+  closed_rty d (<[ a ] ρ [ b ]>).
+Proof.
+  inversion 1. inversion 1. inversion 1.
+  econstructor.
+  econstructor; eauto.
+  simpl. my_set_solver.
+Qed.
